Adapt Isabelle semantics to match Haskell semantics after code review (#35)

semantics-3.0/isabelle/Semantics.thy
@@ -2,14 +2,17 @@ theory Semantics
 imports Main MList SList ListTools
 begin
 
-type_synonym SlotNumber = int
-type_synonym SlotInterval = "SlotNumber \<times> SlotNumber"
+type_synonym Slot = int
+
 type_synonym PubKey = int
+
+type_synonym Ada = int
+
 type_synonym Party = PubKey
-type_synonym NumChoice = int
+type_synonym ChoiceName = int
 type_synonym NumAccount = int
-type_synonym Timeout = SlotNumber
-type_synonym Money = int
+type_synonym Timeout = Slot
+type_synonym Money = Ada
 type_synonym ChosenNum = int
 
 datatype AccountId = AccountId NumAccount Party
@@ -68,7 +71,7 @@ end
 fun accountOwner :: "AccountId \<Rightarrow> Party" where
 "accountOwner (AccountId _ party) = party"
 
-datatype ChoiceId = ChoiceId NumChoice Party
+datatype ChoiceId = ChoiceId ChoiceName Party
 
 (* BEGIN Proof of linorder for ChoiceId *)
 fun less_eq_ChoId :: "ChoiceId \<Rightarrow> ChoiceId \<Rightarrow> bool" where
@@ -121,7 +124,7 @@ qed
 end
 (* END Proof of linorder for ChoiceId *)
 
-datatype OracleId = OracleId PubKey
+(* datatype OracleId = OracleId PubKey
 
 (* BEGIN Proof of linorder for OracleId *)
 fun less_eq_OraId :: "OracleId \<Rightarrow> OracleId \<Rightarrow> bool" where
@@ -171,6 +174,7 @@ next
 qed
 end
 (* END Proof of linorder for OracleId *)
+*)
 
 datatype ValueId = ValueId int
 
@@ -245,6 +249,7 @@ datatype Observation = AndObs Observation Observation
                      | TrueObs
                      | FalseObs
 
+type_synonym SlotInterval = "Slot \<times> Slot"
 type_synonym Bound = "int \<times> int"
 
 fun inBounds :: "ChosenNum \<Rightarrow> Bound list \<Rightarrow> bool" where
@@ -264,16 +269,438 @@ and Contract = Refund
              | When "Case list" Timeout Contract
              | Let ValueId Value Contract
 
-record State = account :: "(AccountId \<times> Money) list"
-               choice :: "(ChoiceId \<times> ChosenNum) list"
+record State = accounts :: "(AccountId \<times> Money) list"
+               choices :: "(ChoiceId \<times> ChosenNum) list"
                boundValues :: "(ValueId \<times> int) list"
-               minSlot :: SlotNumber
+               minSlot :: Slot
 
 record Environment = slotInterval :: SlotInterval
 
 datatype Input = IDeposit AccountId Party Money
                | IChoice ChoiceId ChosenNum
                | INotify
+
+(* Processing of slot interval *)
+datatype IntervalError = InvalidInterval SlotInterval
+                       | IntervalInPastError Slot SlotInterval
+
+datatype IntervalResult = IntervalTrimmed Environment State
+                        | IntervalError IntervalError
+
+fun fixInterval :: "SlotInterval \<Rightarrow> State \<Rightarrow> IntervalResult" where
+"fixInterval (low, high) state =
+   (let curMinSlot = minSlot state in
+    let newLow = max low curMinSlot in
+    let curInterval = (newLow, high) in
+    let env = \<lparr> slotInterval = curInterval \<rparr> in
+    let newState = state \<lparr> minSlot := newLow \<rparr> in
+    (if (high < low)
+     then IntervalError (InvalidInterval (low, high))
+     else (if (high < curMinSlot)
+           then IntervalError (IntervalInPastError curMinSlot (low, high))
+           else IntervalTrimmed env newState)))"
+
+(* EVALUATION *)
+
+fun evalValue :: "Environment \<Rightarrow> State \<Rightarrow> Value \<Rightarrow> int" where
+"evalValue env state (AvailableMoney accId) =
+    findWithDefault 0 accId (accounts state)" |
+"evalValue env state (Constant integer) = integer" |
+"evalValue env state (NegValue val) = evalValue env state val" |
+"evalValue env state (AddValue lhs rhs) =
+    evalValue env state lhs + evalValue env state rhs" |
+"evalValue env state (SubValue lhs rhs) =
+    evalValue env state lhs + evalValue env state rhs" |
+"evalValue env state (ChoiceValue choId defVal) =
+    findWithDefault (evalValue env state defVal) choId (choices state)" |
+"evalValue env state (SlotIntervalStart) = fst (slotInterval env)" |
+"evalValue env state (SlotIntervalEnd) = snd (slotInterval env)" |
+"evalValue env state (UseValue valId) =
+    findWithDefault 0 valId (boundValues state)"
+
+fun evalObservation :: "Environment \<Rightarrow> State \<Rightarrow> Observation \<Rightarrow> bool" where
+"evalObservation env state (AndObs lhs rhs) =
+    (evalObservation env state lhs \<and> evalObservation env state rhs)" |
+"evalObservation env state (OrObs lhs rhs) =
+    (evalObservation env state lhs \<or> evalObservation env state rhs)" |
+"evalObservation env state (NotObs subObs) =
+    (\<not> evalObservation env state subObs)" |
+"evalObservation env state (ChoseSomething choId) =
+    (member choId (choices state))" |
+"evalObservation env state (ValueGE lhs rhs) =
+    (evalValue env state lhs \<ge> evalValue env state rhs)" |
+"evalObservation env state (ValueGT lhs rhs) =
+    (evalValue env state lhs > evalValue env state rhs)" |
+"evalObservation env state (ValueLT lhs rhs) =
+    (evalValue env state lhs < evalValue env state rhs)" |
+"evalObservation env state (ValueLE lhs rhs) =
+    (evalValue env state lhs \<le> evalValue env state rhs)" |
+"evalObservation env state (ValueEQ lhs rhs) =
+    (evalValue env state lhs = evalValue env state rhs)" |
+"evalObservation env state TrueObs = True" |
+"evalObservation env state FalseObs = False"
+
+fun refundOne :: "(AccountId \<times> Money) list \<Rightarrow>
+                  ((Party \<times> Money) \<times> ((AccountId \<times> Money) list)) option" where
+"refundOne ((accId, money)#rest) =
+   (if money > 0 then Some ((accountOwner accId, money), rest) else refundOne rest)" |
+"refundOne [] = None"
+
+lemma refundOneShortens : "refundOne acc = Some (c, nacc) \<Longrightarrow>
+                           length nacc < length acc"
+  apply (induction acc)
+  apply simp
+  by (metis Pair_inject length_Cons less_Suc_eq list.distinct(1)
+            list.inject option.inject refundOne.elims)
+
+datatype Payment = Payment Party Money
+
+datatype ReduceEffect = ReduceNoPayment
+                      | ReduceWithPayment Payment
+
+fun moneyInAccount :: "AccountId \<Rightarrow> ((AccountId \<times> Money) list) \<Rightarrow> Money" where
+"moneyInAccount accId accountsV = findWithDefault 0 accId accountsV"
+
+fun updateMoneyInAccount :: "AccountId \<Rightarrow> Money \<Rightarrow>
+                             ((AccountId \<times> Money) list) \<Rightarrow>
+                             ((AccountId \<times> Money) list)" where
+"updateMoneyInAccount accId money accountsV =
+  (if money \<le> 0
+   then MList.delete accId accountsV
+   else MList.insert accId money accountsV)"
+
+fun addMoneyToAccount :: "AccountId \<Rightarrow> Money \<Rightarrow>
+                          ((AccountId \<times> Money) list) \<Rightarrow>
+                          ((AccountId \<times> Money) list)" where
+"addMoneyToAccount accId money accountsV =
+  (let balance = moneyInAccount accId accountsV in
+   let newBalance = balance + money in
+   if money \<le> 0
+   then accountsV
+   else updateMoneyInAccount accId newBalance accountsV)"
+
+fun giveMoney :: "Payee \<Rightarrow> Money \<Rightarrow>
+                  ((AccountId \<times> Money) list) \<Rightarrow>
+                  (ReduceEffect \<times> ((AccountId \<times> Money) list))" where
+"giveMoney (Party party) money accountsV =
+  (ReduceWithPayment (Payment party money), accountsV)" |
+"giveMoney (Account accId) money accountsV =
+  (let newAccs = addMoneyToAccount accId money accountsV in
+    (ReduceNoPayment, newAccs))"
+
+lemma giveMoneyIncOne : "giveMoney p m a = (e, na) \<Longrightarrow> length na \<le> length a + 1"
+  apply (cases p)
+  apply (cases "m \<le> 0")
+  apply auto
+  by (smt Suc_eq_plus1 delete_length insert_length le_Suc_eq)
+
+(* REDUCE *)
+
+datatype ReduceWarning = ReduceNoWarning
+                       | ReduceNonPositivePay AccountId Payee Money
+                       | ReducePartialPay AccountId Payee Money Money
+                       | ReduceShadowing ValueId int int
+
+datatype ReduceStepResult = Reduced ReduceWarning ReduceEffect State Contract
+                          | NotReduced
+                          | AmbiguousSlotIntervalReductionError
+
+fun reduceContractStep :: "Environment \<Rightarrow> State \<Rightarrow> Contract \<Rightarrow> ReduceStepResult" where
+"reduceContractStep _ state Refund =
+  (case refundOne (accounts state) of
+     Some ((party, money), newAccount) \<Rightarrow>
+       let newState = state \<lparr> accounts := newAccount \<rparr> in
+       Reduced ReduceNoWarning (ReduceWithPayment (Payment party money)) newState Refund
+   | None \<Rightarrow> NotReduced)" |
+"reduceContractStep env state (Pay accId payee val cont) =
+  (let moneyToPay = evalValue env state val in
+   if moneyToPay \<le> 0
+   then Reduced (ReduceNonPositivePay accId payee moneyToPay) ReduceNoPayment state cont
+   else (let balance = moneyInAccount accId (accounts state) in
+        (let paidMoney = min balance moneyToPay in
+         let newBalance = balance - paidMoney in
+         let newAccs = updateMoneyInAccount accId newBalance (accounts state) in
+         let warning = (if paidMoney < moneyToPay
+                        then ReducePartialPay accId payee paidMoney moneyToPay
+                        else ReduceNoWarning) in
+         let (payment, finalAccs) = giveMoney payee paidMoney newAccs in
+         Reduced warning payment (state \<lparr> accounts := finalAccs \<rparr>) cont)))" |
+"reduceContractStep env state (If obs cont1 cont2) =
+  (let cont = (if evalObservation env state obs
+               then cont1
+               else cont2) in
+   Reduced ReduceNoWarning ReduceNoPayment state cont)" |
+"reduceContractStep env state (When _ timeout cont) =
+  (let (startSlot, endSlot) = slotInterval env in
+   if endSlot < timeout
+   then NotReduced
+   else (if timeout \<le> startSlot
+         then Reduced ReduceNoWarning ReduceNoPayment state cont
+         else AmbiguousSlotIntervalReductionError))" |
+"reduceContractStep env state (Let valId val cont) =
+  (let evaluatedValue = evalValue env state val in
+   let boundVals = boundValues state in
+   let newState = state \<lparr> boundValues := MList.insert valId evaluatedValue boundVals \<rparr> in
+   let warn = case lookup valId boundVals of
+                Some oldVal \<Rightarrow> ReduceShadowing valId oldVal evaluatedValue
+              | None \<Rightarrow> ReduceNoWarning in
+   Reduced warn ReduceNoPayment newState cont)"
+
+datatype ReduceResult = ContractQuiescent "ReduceWarning list" "Payment list"
+                                          State Contract
+                      | RRAmbiguousSlotIntervalError
+
+fun evalBound :: "State \<Rightarrow> Contract \<Rightarrow> nat" where
+"evalBound sta cont = length (accounts sta) + 2 * (size cont)"
+
+lemma reduceContractStepReducesSize_Refund_aux :
+  "refundOne (accounts sta) = Some ((party, money), newAccount) \<Longrightarrow>
+   length (accounts (sta\<lparr>accounts := newAccount\<rparr>)) < length (accounts sta)"
+  by (simp add: refundOneShortens)
+
+lemma reduceContractStepReducesSize_Refund_aux2 :
+  "Reduced ReduceNoWarning (ReduceWithPayment (Payment party money))
+          (sta\<lparr>accounts := newAccount\<rparr>) Refund =
+   Reduced twa tef nsta nc \<Longrightarrow>
+   c = Refund \<Longrightarrow>
+   refundOne (accounts sta) = Some ((party, money), newAccount) \<Longrightarrow>
+   length (accounts nsta) + 2 * size nc < length (accounts sta)"
+  apply simp
+  using reduceContractStepReducesSize_Refund_aux by blast
+
+lemma reduceContractStepReducesSize_Refund :
+  "(case a of
+          ((party, money), newAccount) \<Rightarrow>
+            Reduced ReduceNoWarning (ReduceWithPayment (Payment party money))
+             (sta\<lparr>accounts := newAccount\<rparr>) Refund) =
+         Reduced twa tef nsta nc \<Longrightarrow>
+         c = Refund \<Longrightarrow>
+         refundOne (accounts sta) = Some a \<Longrightarrow>
+         length (accounts nsta) + 2 * size nc < length (accounts sta)"
+  apply (cases a)
+  apply simp
+  using reduceContractStepReducesSize_Refund_aux2 by fastforce
+
+lemma zeroMinIfGT : "x > 0 \<Longrightarrow> min 0 x = (0 :: int)"
+  by simp
+
+lemma reduceContractStepReducesSize_Pay_aux :
+  "length z \<le> length x \<Longrightarrow>
+   giveMoney x22 a z = (tef, y) \<Longrightarrow>
+   length y < Suc (Suc (length x))"
+  using giveMoneyIncOne by fastforce
+
+lemma reduceContractStepReducesSize_Pay_aux2 :
+  "giveMoney dst a (MList.delete src x)  = (tef, y) \<Longrightarrow>
+   length y < Suc (Suc (length x))"
+  using delete_length reduceContractStepReducesSize_Pay_aux by blast
+
+lemma reduceContractStepReducesSize_Pay_aux3 :
+  "sta\<lparr>accounts := b\<rparr> = nsta \<Longrightarrow>
+   giveMoney dst a (MList.delete src (accounts sta)) = (tef, b) \<Longrightarrow>
+   length (accounts nsta) < Suc (Suc (length (accounts sta)))"
+  using reduceContractStepReducesSize_Pay_aux2 by auto
+
+lemma reduceContractStepReducesSize_Pay_aux4 :
+  "lookup k x = Some w \<Longrightarrow>
+   giveMoney dst a (MList.insert k v x) = (tef, y) \<Longrightarrow>
+   length y < Suc (Suc (length x))"
+  by (metis insert_existing_length le_refl reduceContractStepReducesSize_Pay_aux)
+
+lemma reduceContractStepReducesSize_Pay_aux5 :
+"sta\<lparr>accounts := ba\<rparr> = nsta \<Longrightarrow>
+ lookup src (accounts sta) = Some a \<Longrightarrow>
+ giveMoney dst (evalValue env sta am) (MList.insert src (a - evalValue env sta am) (accounts sta)) = (tef, ba) \<Longrightarrow>
+ length (accounts nsta) < Suc (Suc (length (accounts sta)))"
+  using reduceContractStepReducesSize_Pay_aux4 by auto
+
+
+lemma reduceContractStepReducesSize_Pay_aux6 :
+  "reduceContractStep env sta c = Reduced twa tef nsta nc \<Longrightarrow>
+   c = Pay src dst am y \<Longrightarrow>
+   evalValue env sta am > 0 \<Longrightarrow>
+   lookup src (accounts sta) = Some a \<Longrightarrow>
+   evalBound nsta nc < evalBound sta c"
+  apply (cases "a < evalValue env sta am")
+  apply (simp add:min_absorb1)
+  apply (cases "giveMoney dst a (MList.delete src (accounts sta))")
+  using reduceContractStepReducesSize_Pay_aux3 apply fastforce
+  apply (cases "a = evalValue env sta am")
+  apply (cases "giveMoney dst (evalValue env sta am) (MList.delete src (accounts sta))")
+  apply (simp add:min_absorb2)
+  using reduceContractStepReducesSize_Pay_aux3 apply blast
+  apply (cases "giveMoney dst (evalValue env sta am) (MList.insert src (a - evalValue env sta am) (accounts sta))")
+  apply (simp add:min_absorb2)
+  using reduceContractStepReducesSize_Pay_aux5 by blast
+
+lemma reduceContractStepReducesSize_Pay :
+  "reduceContractStep env sta c = Reduced twa tef nsta nc \<Longrightarrow>
+   c = Pay src dst am y \<Longrightarrow> evalBound nsta nc < evalBound sta c"
+  apply (cases "evalValue env sta am \<le> 0")
+  apply auto[1]
+  apply (cases "lookup src (accounts sta)")
+  apply (cases "evalValue env sta am > 0")
+  apply (cases "giveMoney dst 0 (MList.delete src (accounts sta))")
+  apply (simp add:zeroMinIfGT)
+  using reduceContractStepReducesSize_Pay_aux3 apply blast
+  apply simp
+  using reduceContractStepReducesSize_Pay_aux6 by auto
+
+lemma reduceContractStepReducesSize_When :
+  "reduceContractStep env sta c = Reduced twa tef nsta nc \<Longrightarrow>
+   c = When cases timeout cont \<Longrightarrow>
+   slotInterval env = (startSlot, endSlot) \<Longrightarrow>
+   evalBound nsta nc < evalBound sta c"
+  apply simp
+  apply (cases "endSlot < timeout")
+  apply simp
+  apply (cases "timeout \<le> startSlot")
+  by simp_all
+
+lemma reduceContractStepReducesSize_Let_aux :
+  "Reduced (ReduceShadowing vId a (evalValue env sta val)) ReduceNoPayment
+         (sta\<lparr>boundValues := MList.insert vId (evalValue env sta val) (boundValues sta)\<rparr>) cont =
+    Reduced twa tef nsta nc \<Longrightarrow>
+   c = Contract.Let vId val cont \<Longrightarrow>
+   lookup vId (boundValues sta) = Some a \<Longrightarrow>
+   evalBound nsta nc < evalBound sta c"
+  by auto  
+
+lemma reduceContractStepReducesSize_Let :
+  "reduceContractStep env sta c = Reduced twa tef nsta nc \<Longrightarrow>
+   c = Contract.Let vId val cont \<Longrightarrow> evalBound nsta nc < evalBound sta c"
+  apply (cases "lookup vId (boundValues sta)")
+  apply auto[1]
+  by (metis ReduceStepResult.inject reduceContractStep.simps(5) reduceContractStepReducesSize_Let_aux)
+
+lemma reduceContractStepReducesSize :
+  "reduceContractStep env sta c = Reduced twa tef nsta nc \<Longrightarrow>
+     (evalBound nsta nc) < (evalBound sta c)"
+  apply (cases c)
+  apply (cases "refundOne (accounts sta)")
+  apply simp
+  apply simp
+  apply (simp add:reduceContractStepReducesSize_Refund)
+  using reduceContractStepReducesSize_Pay apply blast
+  apply auto[1]
+  apply (meson eq_fst_iff reduceContractStepReducesSize_When)
+  using reduceContractStepReducesSize_Let by blast
+
+function (sequential) reductionLoop :: "Environment \<Rightarrow> State \<Rightarrow> Contract \<Rightarrow> ReduceWarning list \<Rightarrow>
+                                        Payment list \<Rightarrow> ReduceResult" where
+"reductionLoop env state contract warnings payments =
+  (case reduceContractStep env state contract of
+     Reduced warning effect newState ncontract \<Rightarrow>
+       let newWarnings = (if warning = ReduceNoWarning
+                          then warnings
+                          else warning # warnings) in
+       let newPayments = (case effect of
+                            ReduceWithPayment payment \<Rightarrow> payment # payments
+                          | ReduceNoPayment \<Rightarrow> payments) in
+       reductionLoop env newState ncontract newWarnings newPayments
+   | AmbiguousSlotIntervalReductionError \<Rightarrow> RRAmbiguousSlotIntervalError
+   | NotReduced \<Rightarrow> ContractQuiescent (rev warnings) (rev payments) state contract)"
+  by pat_completeness auto
+termination reductionLoop
+  apply (relation "measure (\<lambda>(_, (state, (contract, _))) . evalBound state contract)")
+  apply blast
+  using reduceContractStepReducesSize by auto
+
+fun reduceContractUntilQuiescent :: "Environment \<Rightarrow> State \<Rightarrow> Contract \<Rightarrow> ReduceResult" where
+"reduceContractUntilQuiescent env state contract = reductionLoop env state contract [] []"
+
+datatype ApplyResult = Applied State Contract
+                     | ApplyNoMatchError
+
+fun applyCases :: "Environment \<Rightarrow> State \<Rightarrow> Input \<Rightarrow> Case list \<Rightarrow> ApplyResult" where
+"applyCases env state (IDeposit accId1 party1 money)
+            (Cons (Case (Deposit accId2 party2 val) cont) rest) =
+  (let amount = evalValue env state val in
+   let newState = state \<lparr> accounts := addMoneyToAccount accId1 money (accounts state) \<rparr> in
+   if (accId1 = accId2 \<and> party1 = party2 \<and> money = amount)
+   then Applied newState cont
+   else applyCases env state (IDeposit accId1 party1 money) rest)" |
+"applyCases env state (IChoice choId1 choice)
+            (Cons (Case (Choice choId2 bounds) cont) rest) =
+  (let newState = state \<lparr> choices := MList.insert choId1 choice (choices state) \<rparr> in
+   if (choId1 = choId2 \<and> inBounds choice bounds)
+   then Applied newState cont
+   else applyCases env state (IChoice choId1 choice) rest)" |
+"applyCases env state INotify (Cons (Case (Notify obs) cont) rest) =
+  (if evalObservation env state obs
+   then Applied state cont
+   else applyCases env state INotify rest)" |
+"applyCases env state (IDeposit accId1 party1 money) (Cons _ rest) =
+  applyCases env state (IDeposit accId1 party1 money) rest" |
+"applyCases env state (IChoice choId1 choice) (Cons _ rest) =
+  applyCases env state (IChoice choId1 choice) rest" |
+"applyCases env state INotify (Cons _ rest) =
+  applyCases env state INotify rest" |
+"applyCases env state acc Nil = ApplyNoMatchError"
+
+fun applyInput :: "Environment \<Rightarrow> State \<Rightarrow> Input \<Rightarrow> Contract \<Rightarrow> ApplyResult" where
+"applyInput env state input (When cases t cont) = applyCases env state input cases" |
+"applyInput env state input c = ApplyNoMatchError"
+
+datatype ApplyAllResult = ApplyAllSuccess "ReduceWarning list" "Payment list"
+                                     State Contract
+                        | ApplyAllNoMatchError
+                        | ApplyAllAmbiguousSlotIntervalError
+
+fun applyAllLoop :: "Environment \<Rightarrow> State \<Rightarrow> Contract \<Rightarrow> Input list \<Rightarrow>
+                    ReduceWarning list \<Rightarrow> Payment list \<Rightarrow>
+                    ApplyAllResult" where
+"applyAllLoop env state contract inputs warnings payments =
+   (case reduceContractUntilQuiescent env state contract of
+      RRAmbiguousSlotIntervalError \<Rightarrow> ApplyAllAmbiguousSlotIntervalError
+    | ContractQuiescent warns pays curState cont \<Rightarrow>
+       (case inputs of
+          Nil \<Rightarrow> ApplyAllSuccess (warnings @ warns) (payments @ pays) curState cont
+        | Cons input rest \<Rightarrow>
+           (case applyInput env curState input cont of
+              Applied newState cont \<Rightarrow> applyAllLoop env newState cont rest (warnings @ warns) (payments @ pays)
+            | ApplyNoMatchError \<Rightarrow> ApplyAllNoMatchError)))"
+
+fun applyAllInputs :: "Environment \<Rightarrow> State \<Rightarrow> Contract \<Rightarrow> Input list \<Rightarrow>
+                 ApplyAllResult" where
+"applyAllInputs env state contract inputs = applyAllLoop env state contract inputs Nil Nil"
+
+type_synonym TransactionSignatures = "Party list"
+
+datatype TransactionError = TEAmbiguousSlotIntervalError
+                          | TEApplyNoMatchError
+                          | TEIntervalError IntervalError
+                          | TEUselessTransaction
+
+record TransactionOutputRecord = txOutWarnings :: "ReduceWarning list"
+                                 txOutPayments :: "Payment list"
+                                 txOutState :: State
+                                 txOutContract :: Contract
+
+datatype TransactionOutput = TransactionOutput TransactionOutputRecord
+                           | TransactionError TransactionError
+
+record Transaction = interval :: SlotInterval
+                     inputs :: "Input list"
+
+fun computeTransaction :: "Transaction \<Rightarrow> State \<Rightarrow> Contract \<Rightarrow> TransactionOutput" where
+"computeTransaction tx state contract =
+  (let inps = inputs tx in
+   case fixInterval (interval tx) state of
+     IntervalTrimmed env fixSta \<Rightarrow>
+       (case applyAllInputs env fixSta contract inps of
+          ApplyAllSuccess warnings payments newState cont \<Rightarrow>
+            if contract = cont
+            then TransactionError TEUselessTransaction
+            else TransactionOutput \<lparr> txOutWarnings = warnings
+                                   , txOutPayments = payments
+                                   , txOutState = newState
+                                   , txOutContract = cont \<rparr>
+        | ApplyAllNoMatchError \<Rightarrow> TransactionError TEApplyNoMatchError
+        | ApplyAllAmbiguousSlotIntervalError \<Rightarrow> TransactionError TEAmbiguousSlotIntervalError)
+     | IntervalError error \<Rightarrow> TransactionError (TEIntervalError error))"
+
+(* Extra functions *)
 
 type_synonym TransactionOutcomes = "(Party \<times> Money) list"
 
@@ -295,432 +722,8 @@ fun addOutcome :: "Party \<Rightarrow> Money \<Rightarrow> TransactionOutcomes \
 fun combineOutcomes :: "TransactionOutcomes \<Rightarrow> TransactionOutcomes \<Rightarrow> TransactionOutcomes" where
 "combineOutcomes x y = MList.unionWith plus x y"
 
-datatype IntervalError = InvalidInterval SlotInterval
-                       | IntervalInPastError SlotNumber SlotInterval
-
-datatype IntervalResult = IntervalTrimmed Environment State
-                        | IntervalError IntervalError
-
-fun fixInterval :: "SlotInterval \<Rightarrow> State \<Rightarrow> IntervalResult" where
-"fixInterval (l, h) st =
-   (let minSlot = minSlot st in
-    let nl = max l minSlot in
-    let tInt = (nl, h) in
-    let env = \<lparr> slotInterval = tInt \<rparr> in
-    let nst = st \<lparr> minSlot := nl \<rparr> in
-    (if (h < l)
-     then IntervalError (InvalidInterval (l, h))
-     else (if (h < minSlot)
-           then IntervalError (IntervalInPastError minSlot (l, h))
-           else IntervalTrimmed env nst)))"
-
-fun evalValue :: "Environment \<Rightarrow> State \<Rightarrow> Value \<Rightarrow> int" where
-"evalValue env state (AvailableMoney accId) =
-    findWithDefault 0 accId (account state)" |
-"evalValue env state (Constant integer) = integer" |
-"evalValue env state (NegValue val) = evalValue env state val" |
-"evalValue env state (AddValue lhs rhs) =
-    evalValue env state lhs + evalValue env state rhs" |
-"evalValue env state (SubValue lhs rhs) =
-    evalValue env state lhs + evalValue env state rhs" |
-"evalValue env state (ChoiceValue choId defVal) =
-    findWithDefault (evalValue env state defVal) choId (choice state)" |
-"evalValue env state (SlotIntervalStart) = fst (slotInterval env)" |
-"evalValue env state (SlotIntervalEnd) = snd (slotInterval env)" |
-"evalValue env state (UseValue valId) =
-    findWithDefault 0 valId (boundValues state)"
-
-fun evalObservation :: "Environment \<Rightarrow> State \<Rightarrow> Observation \<Rightarrow> bool" where
-"evalObservation env state (AndObs lhs rhs) =
-    (evalObservation env state lhs \<and> evalObservation env state rhs)" |
-"evalObservation env state (OrObs lhs rhs) =
-    (evalObservation env state lhs \<or> evalObservation env state rhs)" |
-"evalObservation env state (NotObs subObs) =
-    (\<not> evalObservation env state subObs)" |
-"evalObservation env state (ChoseSomething choId) =
-    (member choId (choice state))" |
-"evalObservation env state (ValueGE lhs rhs) =
-    (evalValue env state lhs \<ge> evalValue env state rhs)" |
-"evalObservation env state (ValueGT lhs rhs) =
-    (evalValue env state lhs > evalValue env state rhs)" |
-"evalObservation env state (ValueLT lhs rhs) =
-    (evalValue env state lhs < evalValue env state rhs)" |
-"evalObservation env state (ValueLE lhs rhs) =
-    (evalValue env state lhs \<le> evalValue env state rhs)" |
-"evalObservation env state (ValueEQ lhs rhs) =
-    (evalValue env state lhs = evalValue env state rhs)" |
-"evalObservation env state TrueObs = True" |
-"evalObservation env state FalseObs = False"
-
-fun refundOne :: "(AccountId \<times> Money) list \<Rightarrow>
-                  ((Party \<times> Money) \<times> ((AccountId \<times> Money) list)) option" where
-"refundOne ((accId, mon)#rest) =
-   (if mon > 0 then Some ((accountOwner accId, mon), rest) else refundOne rest)" |
-"refundOne [] = None"
-
-lemma refundOneShortens : "refundOne acc = Some (c, nacc) \<Longrightarrow>
-                           length nacc < length acc"
-  apply (induction acc)
-  apply simp
-  by (metis Pair_inject length_Cons less_Suc_eq list.distinct(1)
-            list.inject option.inject refundOne.elims)
-
-fun moneyInAccount :: "((AccountId \<times> Money) list) \<Rightarrow> AccountId \<Rightarrow> Money" where
-"moneyInAccount accs accId = findWithDefault 0 accId accs"
-
-fun updateMoneyInAccount :: "((AccountId \<times> Money) list) \<Rightarrow> AccountId \<Rightarrow>
-                             Money \<Rightarrow> ((AccountId \<times> Money) list)" where
-"updateMoneyInAccount accs accId mon =
-  (if mon \<le> 0
-   then MList.delete accId accs
-   else MList.insert accId mon accs)"
-
-fun withdrawMoneyFromAccount :: "((AccountId \<times> Money) list) \<Rightarrow> AccountId \<Rightarrow>
-                                 Money \<Rightarrow> (Money \<times> ((AccountId \<times> Money) list))" where
-"withdrawMoneyFromAccount accs accId mon =
-  (let avMoney = moneyInAccount accs accId in
-   case min avMoney mon of withdrawnMoney \<Rightarrow>
-   let newAvMoney = avMoney - withdrawnMoney in
-   let newAcc = updateMoneyInAccount accs accId newAvMoney in
-   (withdrawnMoney, newAcc))"
-
-fun addMoneyToAccount :: "((AccountId \<times> Money) list) \<Rightarrow> AccountId \<Rightarrow>
-                          Money \<Rightarrow> ((AccountId \<times> Money) list)" where
-"addMoneyToAccount accs accId mon =
-  (let avMoney = moneyInAccount accs accId in
-   let newAvMoney = avMoney + mon in
-   if mon \<le> 0
-   then accs
-   else updateMoneyInAccount accs accId newAvMoney)"
-
-datatype ReduceWarning = ReduceNoWarning
-                       | ReduceNonPositivePay AccountId Payee Money
-                       | ReducePartialPay AccountId Payee Money Money
-                       | ReduceShadowing ValueId int int
-
-datatype ReduceEffect = ReduceNoEffect
-                      | ReduceNormalPay Party Money
-
-datatype ReduceError = ReduceAmbiguousSlotInterval
-
-datatype ReduceResult = Reduced ReduceWarning ReduceEffect State Contract
-                      | NotReduced
-                      | ReduceError ReduceError
-
-fun giveMoney :: "((AccountId \<times> Money) list) \<Rightarrow> Payee \<Rightarrow>
-                  Money \<Rightarrow> (ReduceEffect \<times> ((AccountId \<times> Money) list))" where
-"giveMoney accs (Party party) mon = (ReduceNormalPay party mon, accs)" |
-"giveMoney accs (Account accId) mon =
-  (let newAccs = addMoneyToAccount accs accId mon in
-    (ReduceNoEffect, newAccs))"
-
-lemma giveMoneyIncOne : "giveMoney a p m = (e, na) \<Longrightarrow> length na \<le> length a + 1"
-  apply (cases p)
-  apply (cases "m \<le> 0")
-  apply auto
-  by (smt Suc_eq_plus1 delete_length insert_length le_Suc_eq)
-
-fun reduce :: "Environment \<Rightarrow> State \<Rightarrow> Contract \<Rightarrow> ReduceResult" where
-"reduce _ state Refund =
-  (case refundOne (account state) of
-     Some ((party, money), newAccount) \<Rightarrow>
-       let newState = state \<lparr> account := newAccount \<rparr> in
-       Reduced ReduceNoWarning (ReduceNormalPay party money) newState Refund
-   | None \<Rightarrow> NotReduced)" |
-"reduce env state (Pay accId payee val nc) =
-  (case evalValue env state val of mon \<Rightarrow>
-   let (paidMon, newAccs) = withdrawMoneyFromAccount (account state) accId mon in
-   let noMonWarn = (if paidMon < mon
-                    then ReducePartialPay accId payee paidMon mon
-                    else ReduceNoWarning) in
-   let (payEffect, finalAccs) = giveMoney newAccs payee paidMon in
-   if mon \<le> 0
-   then Reduced (ReduceNonPositivePay accId payee mon) ReduceNoEffect state nc
-   else Reduced noMonWarn payEffect (state \<lparr> account := finalAccs \<rparr>) nc)" |
-"reduce env state (If obs cont1 cont2) =
-  (let nc = (if evalObservation env state obs
-             then cont1
-             else cont2) in
-   Reduced ReduceNoWarning ReduceNoEffect state nc)" |
-"reduce env state (When _ timeout c) =
-  (let (startSlot, endSlot) = slotInterval env in
-   if endSlot < timeout
-   then NotReduced
-   else (if startSlot \<ge> timeout
-         then Reduced ReduceNoWarning ReduceNoEffect state c
-         else ReduceError ReduceAmbiguousSlotInterval))" |
-"reduce env state (Let valId val cont) =
-  (let sv = boundValues state in
-   case evalValue env state val of evVal \<Rightarrow>
-   let nsv = MList.insert valId evVal sv in
-   let ns = state \<lparr> boundValues := nsv \<rparr> in
-   let warn = case lookup valId sv of
-                Some oldVal \<Rightarrow> ReduceShadowing valId oldVal evVal
-              | None \<Rightarrow> ReduceNoWarning in
-   Reduced warn ReduceNoEffect ns cont)"
-
-datatype ReduceAllResult = ReducedAll "ReduceWarning list" "ReduceEffect list"
-                                      State Contract
-                         | ReduceAllError ReduceError
-
-fun evalBound :: "State \<Rightarrow> Contract \<Rightarrow> nat" where
-"evalBound sta cont = length (account sta) + 2 * (size cont)"
-
-lemma reduceReducesSize_Refund_aux :
-  "refundOne (account sta) = Some ((party, money), newAccount) \<Longrightarrow>
-   length (account (sta\<lparr>account := newAccount\<rparr>)) < length (account sta)"
-  by (simp add: refundOneShortens)
-
-lemma reduceReducesSize_Refund_aux2 :
-  "Reduced ReduceNoWarning (ReduceNormalPay party money)
-          (sta\<lparr>account := newAccount\<rparr>) Refund =
-   Reduced twa tef nsta nc \<Longrightarrow>
-   c = Refund \<Longrightarrow>
-   refundOne (account sta) = Some ((party, money), newAccount) \<Longrightarrow>
-   length (account nsta) + 2 * size nc < length (account sta)"
-  apply simp
-  using reduceReducesSize_Refund_aux by blast
-
-lemma reduceReducesSize_Refund_aux3 :
-  "(case a of
-          ((party, money), newAccount) \<Rightarrow>
-            Reduced ReduceNoWarning (ReduceNormalPay party money)
-             (sta\<lparr>account := newAccount\<rparr>) Refund) =
-         Reduced twa tef nsta nc \<Longrightarrow>
-         c = Refund \<Longrightarrow>
-         refundOne (account sta) = Some a \<Longrightarrow>
-         length (account nsta) + 2 * size nc < length (account sta)"
-  apply (cases a)
-  apply simp
-  using reduceReducesSize_Refund_aux2 by fastforce
-
-lemma zeroMinIfGT : "x > 0 \<Longrightarrow> min 0 x = (0 :: int)"
-  by simp
-
-lemma reduceReducesSize_Pay_aux :
-  "length z \<le> length x \<Longrightarrow>
-   giveMoney z x22 a = (tef, y) \<Longrightarrow>
-   length y < Suc (Suc (length x))"
-  using giveMoneyIncOne by fastforce
-
-lemma reduceReducesSize_Pay_aux2 :
-  "giveMoney (MList.delete src x) dst a = (tef, y) \<Longrightarrow>
-   length y < Suc (Suc (length x))"
-  using delete_length reduceReducesSize_Pay_aux by blast
-
-lemma reduceReducesSize_Pay_aux3 :
-  "sta\<lparr>account := b\<rparr> = nsta \<Longrightarrow>
-   giveMoney (MList.delete src (account sta)) dst a = (tef, b) \<Longrightarrow>
-   length (account nsta) < Suc (Suc (length (account sta)))"
-  using reduceReducesSize_Pay_aux2 by auto
-
-lemma reduceReducesSize_Pay_aux4 :
-  "lookup k x = Some w \<Longrightarrow>
-   giveMoney (MList.insert k v x) dst a = (tef, y) \<Longrightarrow>
-   length y < Suc (Suc (length x))"
-  by (metis insert_existing_length le_refl reduceReducesSize_Pay_aux)
-
-lemma reduceReducesSize_Pay_aux5 :
-"sta\<lparr>account := ba\<rparr> = nsta \<Longrightarrow>
- lookup src (account sta) = Some a \<Longrightarrow>
- giveMoney (MList.insert src (a - evalValue env sta am) (account sta)) dst (evalValue env sta am) = (tef, ba) \<Longrightarrow>
- length (account nsta) < Suc (Suc (length (account sta)))"
-  using reduceReducesSize_Pay_aux4 by auto
-
-lemma not_leq_min : "(\<not> (a \<le> x)) \<Longrightarrow> \<not> (min a (x::int) < x)"
-  by simp
-
-lemma not_leq_min2 : "(\<not> (a \<le> x)) \<Longrightarrow> (min a (x::int) = x)"
-  by auto
-
-lemma reduceReducesSize_Pay_aux6 :
-  "reduce env sta c = Reduced twa tef nsta nc \<Longrightarrow>
-   c = Pay src dst am y \<Longrightarrow>
-   lookup src (account sta) = Some a \<Longrightarrow>
-   evalBound nsta nc < evalBound sta c"
-  apply (cases "giveMoney (MList.delete src (account sta)) dst 0")
-  apply (cases "a \<le> evalValue env sta am")
-  apply (cases "a = evalValue env sta am")
-  apply (cases "giveMoney (MList.delete src (account sta)) dst
-                          (evalValue env sta am)")
-  apply (simp add:zeroMinIfGT)
-  apply (cases "evalValue env sta am \<le> 0")
-  apply simp
-  apply simp
-  using reduceReducesSize_Pay_aux3 apply blast
-  apply (simp add:min_absorb1)
-  apply (cases "giveMoney (MList.delete src (account sta)) dst
-                          a")
-  apply (cases "evalValue env sta am \<le> 0")
-  apply simp
-  apply simp
-  using reduceReducesSize_Pay_aux3 apply blast
-  apply (cases "evalValue env sta am \<le> 0")
-   apply (cases "giveMoney (MList.insert src (a - evalValue env sta am) (account sta)) dst
-                           (evalValue env sta am)")
-  apply (simp add:not_leq_min not_leq_min2)
-  apply (cases "giveMoney (MList.insert src (a - evalValue env sta am) (account sta)) dst
-                          (evalValue env sta am)")
-  apply (simp add:not_leq_min not_leq_min2)
-  using reduceReducesSize_Pay_aux5 by blast
-
-lemma reduceReducesSize_Pay_aux7 :
-  "reduce env sta c = Reduced twa tef nsta nc \<Longrightarrow>
-   c = Pay src dst am y \<Longrightarrow> evalBound nsta nc < evalBound sta c"
-  apply (cases "lookup src (account sta)")
-  apply (cases "evalValue env sta am > 0")
-  apply (cases "giveMoney (MList.delete src (account sta)) dst 0")
-  apply (simp add:zeroMinIfGT)
-  using reduceReducesSize_Pay_aux3 apply blast
-  apply (cases "evalValue env sta am > 0")
-  apply blast
-  apply auto[1]
-  by (metis reduceReducesSize_Pay_aux6)
-
-lemma reduceReducesSize_When_aux :
-  "reduce env sta c = Reduced twa tef nsta nc \<Longrightarrow>
-   c = When cases timeout cont \<Longrightarrow>
-   slotInterval env = (startSlot, endSlot) \<Longrightarrow>
-   evalBound nsta nc < evalBound sta c"
-  apply simp
-  apply (cases "endSlot < timeout")
-  apply simp
-  apply (cases "timeout \<le> startSlot")
-  by simp_all
-
-lemma reduceReducesSize_Let_aux :
-  "reduce env sta c = Reduced twa tef nsta nc \<Longrightarrow>
-   c = Contract.Let vId val cont \<Longrightarrow> evalBound nsta nc < evalBound sta c"
-  apply (cases "lookup vId (boundValues sta)")
-  by auto
-
-lemma reduceReducesSize :
-  "reduce env sta c = Reduced twa tef nsta nc \<Longrightarrow>
-     (evalBound nsta nc) < (evalBound sta c)"
-  apply (cases c)
-  apply (cases "refundOne (account sta)")
-  apply simp
-  apply simp
-  apply (simp add:reduceReducesSize_Refund_aux3)
-  using reduceReducesSize_Pay_aux7 apply blast
-  apply auto[1]
-  apply (meson eq_fst_iff reduceReducesSize_When_aux)
-  using reduceReducesSize_Let_aux by blast
-
-function (sequential) reduceAllAux :: "Environment \<Rightarrow> State \<Rightarrow> Contract \<Rightarrow> ReduceWarning list \<Rightarrow>
-                                       ReduceEffect list \<Rightarrow> ReduceAllResult" where
-"reduceAllAux env sta c wa ef =
-  (case reduce env sta c of
-     Reduced twa tef nsta nc \<Rightarrow>
-       let nwa = (if twa = ReduceNoWarning
-                  then wa
-                  else twa # wa) in
-       let nef = (if tef = ReduceNoEffect
-                  then ef
-                  else tef # ef) in
-       reduceAllAux env nsta nc nwa nef
-   | ReduceError err \<Rightarrow> ReduceAllError err
-   | NotReduced \<Rightarrow> ReducedAll (rev wa) (rev ef) sta c)"
-  by pat_completeness auto
-termination reduceAllAux
-  apply (relation "measure (\<lambda>(_, (st, (c, _))) . evalBound st c)")
-  apply blast
-  using reduceReducesSize by auto
-
-fun reduceAll :: "Environment \<Rightarrow> State \<Rightarrow> Contract \<Rightarrow> ReduceAllResult" where
-"reduceAll env sta c = reduceAllAux env sta c [] []"
-
-datatype ApplyError = ApplyNoMatch
-
-datatype ApplyResult = Applied State Contract
-                     | ApplyError ApplyError
-
-fun applyCases :: "Environment \<Rightarrow> State \<Rightarrow> Input \<Rightarrow> Case list \<Rightarrow> ApplyResult" where
-"applyCases env state (IDeposit accId1 party1 mon1)
-            (Cons (Case (Deposit accId2 party2 val2) nc) t) =
-  (case evalValue env state val2 of mon2 \<Rightarrow>
-   let accs = account state in
-   let newAccs = addMoneyToAccount accs accId1 mon1 in
-   let newState = state \<lparr> account := newAccs \<rparr> in
-   if (accId1 = accId2 \<and> party1 = party2 \<and> mon1 = mon2)
-   then Applied newState nc
-   else applyCases env state (IDeposit accId1 party1 mon1) t)" |
-"applyCases env state (IChoice choId1 cho1)
-            (Cons (Case (Choice choId2 bounds2) nc) t) =
-  (let newState = state \<lparr> choice := MList.insert choId1 cho1 (choice state) \<rparr> in
-   if (choId1 = choId2 \<and> inBounds cho1 bounds2)
-   then Applied newState nc
-   else applyCases env state (IChoice choId1 cho1) t)" |
-"applyCases env state INotify (Cons (Case (Notify obs) nc) t) =
-  (if evalObservation env state obs
-   then Applied state nc
-   else applyCases env state INotify t)" |
-"applyCases env state (IDeposit accId1 party1 mon1) (Cons h t) =
-  applyCases env state (IDeposit accId1 party1 mon1) t" |
-"applyCases env state (IChoice choId1 cho1) (Cons h t) =
-  applyCases env state (IChoice choId1 cho1) t" |
-"applyCases env state INotify (Cons h t) =
-  applyCases env state INotify t" |
-"applyCases env state acc Nil = ApplyError ApplyNoMatch"
-
-fun applyM :: "Environment \<Rightarrow> State \<Rightarrow> Input \<Rightarrow> Contract \<Rightarrow> ApplyResult" where
-"applyM env state act (When cases t cont) = applyCases env state act cases" |
-"applyM env state act c = ApplyError ApplyNoMatch"
-
-datatype ApplyAllResult = AppliedAll "ReduceWarning list" "ReduceEffect list"
-                                     State Contract
-                        | AAApplyError ApplyError
-                        | AAReduceError ReduceError
-
-fun applyAllAux :: "Environment \<Rightarrow> State \<Rightarrow> Contract \<Rightarrow> Input list \<Rightarrow>
-                    ReduceWarning list \<Rightarrow> ReduceEffect list \<Rightarrow>
-                    ApplyAllResult" where
-"applyAllAux env state c l wa ef =
-   (case reduceAll env state c of
-      ReduceAllError raerr \<Rightarrow> AAReduceError raerr
-    | ReducedAll twa tef tstate tc \<Rightarrow>
-       (case l of
-          Nil \<Rightarrow> AppliedAll (wa @ twa) (ef @ tef) tstate tc
-        | Cons h t \<Rightarrow>
-           (case applyM env tstate h tc of
-              Applied nst nc \<Rightarrow> applyAllAux env nst nc t (wa @ twa) (ef @ tef)
-            | ApplyError aeerr \<Rightarrow> AAApplyError aeerr)))"
-
-fun applyAll :: "Environment \<Rightarrow> State \<Rightarrow> Contract \<Rightarrow> Input list \<Rightarrow>
-                 ApplyAllResult" where
-"applyAll env state c l = applyAllAux env state c l Nil Nil"
-
-type_synonym TransactionSignatures = "Party list"
-
-datatype ProcessError = PEReduceError ReduceError
-                      | PEApplyError ApplyError
-                      | PEIntervalError IntervalError
-                      | PEUselessTransaction
-
-type_synonym ProcessWarning = ReduceWarning
-type_synonym ProcessEffect = ReduceEffect
-
-datatype ProcessResult = Processed "ProcessWarning list"
-                                   "ProcessEffect list"
-                                   TransactionSignatures
-                                   TransactionOutcomes
-                                   State
-                                   Contract
-                       | ProcessError ProcessError
-
-record Transaction = interval :: SlotInterval
-                     inputs :: "Input list"
-
-fun addSig :: "Party list \<Rightarrow> Input \<Rightarrow> Party list" where
-"addSig acc (IDeposit _ p _) = SList.insert p acc" |
-"addSig acc (IChoice (ChoiceId _ p) _) = SList.insert p acc" |
-"addSig acc INotify = acc"
-
-fun getSignatures :: "Input list \<Rightarrow> TransactionSignatures" where
-"getSignatures l = foldl addSig SList.empty l"
-
 fun getPartiesFromReduceEffect :: "ReduceEffect list \<Rightarrow> (Party \<times> Money) list" where
-"getPartiesFromReduceEffect (Cons (ReduceNormalPay p m) t) =
+"getPartiesFromReduceEffect (Cons (ReduceWithPayment (Payment p m)) t) =
    Cons (p, -m) (getPartiesFromReduceEffect t)" |
 "getPartiesFromReduceEffect (Cons x t) = getPartiesFromReduceEffect t" |
 "getPartiesFromReduceEffect Nil = Nil"
@@ -736,20 +739,12 @@ fun getOutcomes :: "ReduceEffect list \<Rightarrow> Input list \<Rightarrow> Tra
    foldl (\<lambda> acc (p, m) . addOutcome p m acc) emptyOutcome
          ((getPartiesFromReduceEffect eff) @ (getPartiesFromInput inp))"
 
-fun process :: "Transaction \<Rightarrow> State \<Rightarrow> Contract \<Rightarrow> ProcessResult" where
-"process tra sta c =
-  (let inps = inputs tra in
-   case fixInterval (interval tra) sta of
-     IntervalTrimmed env fixSta \<Rightarrow>
-       (case applyAll env fixSta c inps of
-          AppliedAll wa ef nsta ncon \<Rightarrow>
-            let sigs = getSignatures inps in
-            let outcomes = getOutcomes ef inps in
-            if c = ncon
-            then ProcessError PEUselessTransaction
-            else Processed wa ef sigs outcomes nsta ncon
-        | AAApplyError aperr \<Rightarrow> ProcessError (PEApplyError aperr)
-        | AAReduceError reerr \<Rightarrow> ProcessError (PEReduceError reerr))
-     | IntervalError intErr \<Rightarrow> ProcessError (PEIntervalError intErr))"
+fun addSig :: "Party list \<Rightarrow> Input \<Rightarrow> Party list" where
+"addSig acc (IDeposit _ p _) = SList.insert p acc" |
+"addSig acc (IChoice (ChoiceId _ p) _) = SList.insert p acc" |
+"addSig acc INotify = acc"
+
+fun getSignatures :: "Input list \<Rightarrow> TransactionSignatures" where
+"getSignatures l = foldl addSig SList.empty l"
 
 end
